import cleanup

dfy_model/MultiplyExpr256.dfy
@@ -1,4 +1,4 @@
-include "../dfy_model/NativeTypes.dfy"
+include "NativeTypes.dfy"
 
 module MultiplyExpr256 {
     import opened NativeTypes
@@ -9,26 +9,26 @@ module MultiplyExpr256 {
         [1, 2, 3, 4]
 
     const B : int := UINT64_MAX as int + 1;
-    const B2 : int;
+    const B2 : int := B * B;
     const B3 : int;
     const B4 : int;
     const B5 : int;
     const B6 : int;
     const B7 : int;
 
-    function method lh(x: uint128) : uint64
+    function method lh(x: uint256) : uint128
         ensures flh(x) == lh(x) as int;
 
     function flh(x: int) : (r: int)
 
- 	function method uh(x: uint128) : (r: uint64)
+ 	function method uh(x: uint256) : (r: uint128)
         ensures fuh(x) == uh(x) as int;
 
     function fuh(x: int) : (r: int)
 
- 	lemma split_lemma(x: uint128)
- 	 	ensures flh(x) * B + flh(x) == x;
- 	 	ensures flh(x) == x % B;
+ 	lemma split_lemma(x: uint256)
+ 	 	ensures flh(x) * B2 + flh(x) == x;
+ 	 	ensures flh(x) == x % B2;
 
     method mul_limb(a: uint64, b: uint64)
         returns (c: uint128)
@@ -41,18 +41,22 @@ module MultiplyExpr256 {
     // {
     //     wr[0] as int + wr[1] as int * BASE + 
     // }
+
     method test_full_mul(a : wide_register, b : wide_register)
-        returns (c : wide_register, d : wide_register)
+        returns (c_01: uint128, c_23: uint128, d_01: uint128, d_23: uint128)
     {
         var p0 :uint128 := mul_limb(a[0], b[0]);
         var p1 :uint128 := mul_limb(a[1], b[0]);
         var p2 :uint128 := mul_limb(a[0], b[1]);
 
-        var t0: uint256 := p0 + p1 * B + p2 * B;
+        var t0 :uint256 := p0 + p1 * B + p2 * B;
+        // c_01 :=
     
         var p3 :uint128 := mul_limb(a[2], b[0]);
         var p4 :uint128 := mul_limb(a[1], b[1]);
         var p5 :uint128 := mul_limb(a[0], b[2]);
+
+        var t1 :uint256 := p0 + p1 * B + p2 * B;
 
         var p6 :uint128 := mul_limb(a[3], b[0]);
         var p7 :uint128 := mul_limb(a[2], b[1]);
